formal/fstar/ocaml-patches.sh
@@ -214,24 +214,24 @@ let eval_expr_fwd_ref : (expr -> RDF_Graph_Executable.solution_mapping -> eval_r
   ref (fun _ _ -> failwith \"eval_expr_ebv not yet wired\")
 let eval_expr_fwd_ref : (expr -> RDF_Graph_Executable.solution_mapping -> eval_result) ref =
   ref (fun _ _ -> failwith \"eval_expr_fwd not yet wired\")
-let eval_exists_fwd_ref : (group_graph_pattern -> RDF_Graph_Executable.solution_mapping -> RDF_Graph_Executable.rdf_graph -> Prims.bool) ref =
-  ref (fun _ _ _ -> false)
+let eval_exists_fwd_ref : (group_graph_pattern -> RDF_Graph_Executable.solution_mapping -> RDF_Graph_Executable.rdf_graph -> RDF_Graph_Executable.rdf_dataset -> Prims.bool) ref =
+  ref (fun _ _ _ _ -> false)
 let eval_property_path_fwd_ref : (property_path -> RDF_Graph_Executable.rdf_graph -> (RDF_Graph_Executable.rdf_term * RDF_Graph_Executable.rdf_term) Prims.list) ref =
   ref (fun _ _ -> [])
-let eval_subselect_fwd_ref : (query -> RDF_Graph_Executable.rdf_graph -> solution_sequence) ref =
-  ref (fun _ _ -> [])'''
+let eval_subselect_fwd_ref : (query -> RDF_Graph_Executable.rdf_graph -> RDF_Graph_Executable.rdf_dataset -> solution_sequence) ref =
+  ref (fun _ _ _ -> [])'''
 )
 
 # Replace eval_exists_fwd failwith body with forward ref dispatch
 content = content.replace(
     '''  failwith \"Not yet implemented: SPARQL11.Algebra.eval_exists_fwd\"''',
-    '''  !eval_exists_fwd_ref uu___ uu___1 uu___2'''
+    '''  !eval_exists_fwd_ref uu___ uu___1 uu___2 uu___3'''
 )
 
 # 2e. Wire eval_subselect_fwd to the concrete eval_select_query.
 content = content.replace(
     '''  failwith \"Not yet implemented: SPARQL11.Algebra.eval_subselect_fwd\"''',
-    '''  !eval_subselect_fwd_ref uu___ uu___1'''
+    '''  !eval_subselect_fwd_ref uu___ uu___1 uu___2'''
 )
 
 # 2d. Wire eval_property_path_fwd to the concrete eval_property_path.
